iris/UkCatFEntries.v
@@ -115,7 +115,8 @@ Section UkCatFEntries.
   Local Notation LEND qf sf pn gp w A X ds xs Q :=
     (cif_catf_lend cf rf g M V G v I sR lR L TERM TOK dep γc γm qf sf pn gp w A X ds xs Q).
 
-  (* THE ENTRY, at either state of `f` *)
+  (* THE ENTRY, at either state of the file [f] -- any name of the class
+     (cut W3) *)
   Lemma pse_catf_image_entry_gen (f : list (bv 8)) (Mn : gmap Z (bv 8)) (sv t : Z)
       (gn : nat -> bv 8) (sts : list fdstate) (cw : Z) (cs : gset gname) (pidv : mword 32)
       (Q : Z -> iProp Σ) (pn : pnames) (gp : pipe_names) (w : wid)
@@ -135,19 +136,18 @@ Section UkCatFEntries.
       (LEND qf sf pn gp w A X ds xs Q) uslot.
   Proof using HL31 Hadmit Hcons Heq Hext Hfc Hkill HlR Hplok Hsup cifRegG0 dep_tl ufdG0.
     intros HQc Hf Hok Hnode Hab Hfdl Hcw Hl1 Hl2 Hcase.
-    rewrite /uname in Hf. subst f.
     iIntros "#Hnpw #Hdep".
     set (wv := fun _ : nat => UDProd pn gp w A X).
     set (kds := [(0%nat, UDProd pn gp w A X)]).
     set (files := files_of (dst_content sf)).
-    assert (Hfs : files fname_f = snd <$> sf !! fname_f) by exact (dst_content_lookup sf fname_f).
-    assert (Hc : conforms (catp_env (DProd [L; []] xs ds) files [fname_f])
-                   (cat_tree (prod_words (PrCatF fname_f)))).
-    { change (cat_tree (prod_words (PrCatF fname_f))) with (cat_tree [sb "cat"; fname_f]).
+    assert (Hfs : files f = snd <$> sf !! f) by exact (dst_content_lookup sf f).
+    assert (Hc : conforms (catp_env (DProd [L; []] xs ds) files [f])
+                   (cat_tree (prod_words (PrCatF f)))).
+    { change (cat_tree (prod_words (PrCatF f))) with (cat_tree [sb "cat"; f]).
       destruct Hcase as [(Hs & Hx & Hn & Hw) | (Hs & Hx)].
-      - apply (cat_file_prod_conforms_gen fname_f L); [rewrite Hfs; exact Hs | by left
+      - apply (cat_file_prod_conforms_gen f L); [rewrite Hfs; exact Hs | by left
                                                      | by right; left | exact Hx | exact Hn | exact Hw].
-      - apply (cat_file_prod_absent_conforms_gen fname_f); [rewrite Hfs Hs; reflexivity
+      - apply (cat_file_prod_absent_conforms_gen f); [rewrite Hfs Hs; reflexivity
                                                            | by right; left | exact Hx]. }
     rewrite /image_entry.
     iIntros "!>" (na alen afun W') "%Hokk %Hcwv %Hlz %Hch %Hpid %Hargs Hmp HPay".
@@ -156,9 +156,9 @@ Section UkCatFEntries.
     set (If := fun (N' : uk_names Σ) (Hpq : ukn_pay N' = Q) =>
                  cfe_iface γreg kds (cfe_nodup0 _) (cfe_kdp0 pn gp w A X) qf sf N'
                    (ukn_const_of_eq N' Q Hpq HQc)).
-    iPoseProof (cat_image_entry_env_c (PS := PS) (prod_words (PrCatF fname_f)) Mn sv t gn sts cw cs
+    iPoseProof (cat_image_entry_env_c (PS := PS) (prod_words (PrCatF f)) Mn sv t gn sts cw cs
                   pidv Q (own γreg (cif_pool ∅ wv) ∗ LEND qf sf pn gp w A X ds xs Q)%I
-                  If (catp_env (DProd [L; []] xs ds) files [fname_f]) {[0%nat]}
+                  If (catp_env (DProd [L; []] xs ds) files [f]) {[0%nat]}
                   Hok Hnode Hab Hfdl Hc (cat_tree_safe _ _) (cfe_dp0 _)
                   with "[] Hnpw Hdep") as "#He".
     { iIntros "!>" (N' Hpq) "Hstd Hcwd [Hpool Hlend]".
@@ -169,8 +169,8 @@ Section UkCatFEntries.
                 (HNc := ukn_const_of_eq N' Q Hpq HQc)
                 (cat_stub_read N') (cat_stub_write N') (cat_stub_open N')
                 (cat_stub_close N') (cat_stub_exit N') γreg kds (cfe_nodup0 _)
-                (cfe_kdp0 pn gp w A X) qf sf pn gp w A X ds xs (take NSTD sts) rb1 rb2 wv files
-                eq_refl eq_refl Hl1 Hl2 Hfs
+                (cfe_kdp0 pn gp w A X) qf sf pn gp w A X ds xs (take NSTD sts) rb1 rb2 wv files f
+                eq_refl eq_refl Hl1 Hl2 Hf Hfs
                 with "Hstd Hcwd Hpool Hlend"). }
     iApply ("He" $! na alen afun W' with "[%] [%] [%] [%] [%] [%] Hmp [Hpool HPay]");
       [ exact Hokk | exact Hcwv | exact Hlz | exact Hch | exact Hpid | exact Hargs | ].
